

$$(3) \int \frac{x^2+1}{(x^2-2x+2)^2} dx$$

$$= \int \frac{x^2+1}{((x-1)^2+1)^2} dx$$

$$= \int \frac{(u+1)^2+1}{(u^2+1)^2} du$$

$$u = x-1$$

$$u = \tan \theta$$

$$\sqrt{1+u^2} \rightarrow \text{Trig Sub}$$

$$= \int \frac{(\tan \theta + 1)^2 + 1}{\sec^4 \theta} \sec^2 \theta d\theta$$

$$= \int \cos^2 \theta [(\tan \theta + 1)^2 + 1] d\theta$$

$$= \int \cos^2 \theta d\theta + \int \cos^2 \theta (\tan \theta + 1)^2 d\theta$$

$$= \int \cos^2 \theta d\theta + \int (\sin \theta + \cos \theta)^2 d\theta$$

$$= \int \cos^2 \theta d\theta + \int \sin^2 \theta d\theta + \int \cos^2 \theta d\theta + \int 2 \sin \theta \cos \theta d\theta$$

$$\int 1 d\theta$$

$$= \int 1 d\theta + \int \frac{\cos 2\theta + 1}{2} d\theta + \int \sin 2\theta d\theta$$

$$= \theta + \frac{\sin 2\theta}{2} + \frac{\theta}{2} - \frac{\cos 2\theta}{2} + c$$

$$= \frac{3\theta}{2} + \frac{\sin 2\theta}{2} - \frac{\cos 2\theta}{2} + c$$

$$= \frac{3 \tan^{-1} u}{2} + \frac{2u}{1+u^2} - \frac{1-u^2}{1+u^2} + c$$

$$= \frac{3 \tan^{-1} u + \frac{u^2+u-1}{1+u^2}}{2} + c$$

$$= \frac{3 \tan^{-1} u + \frac{u-2}{1+u^2}}{2} + \frac{1}{2} + c$$

$$= \frac{3 \tan^{-1}(x-1) + \frac{x-3}{1+(x-1)^2}}{2} + c$$